main/lf/terse/lean/LF/Preface.lean
@@ -246,7 +246,7 @@ import LF.SFLCompat
 -- ### System Requirements
 
 -- Lean runs on Windows, Linux, and MacOS. The files in this
--- book have been tested with Lean version `4.32.0`.
+-- book have been tested with Lean version `4.33.0`.
 
 -- ### Installation
 
